passes: Verify `InlineLastBlock`

src/Passes/SimplifyEmptyBlocks.dfy
@@ -10,7 +10,7 @@ include "../Transforms/BottomUp.dfy"
 include "EliminateNegatedBinops.dfy"
 
 module Bootstrap.Passes.SimplifyEmptyBlocks {
-  // This module implements a simple pass, by which we simplify the empty blocks in a program.
+  // This module implements a simple pass, which simplifies the empty blocks in a program.
   //
   // We do the following:
   // 1. we filter the expressions which are empty blocks in blocks of expressions (``FilterEmptyBlocks``):
@@ -55,6 +55,8 @@ module Bootstrap.Passes.SimplifyEmptyBlocks {
   // some blocks might lead to the simplification of some `if then else` branches which might in
   // turn lead to the simplification of other blocks, etc.
   //
+  // Rk.: pass 3. removes expressions which might fail  a pass like 3. is correct, because following definition of ``EqInterp`` 
+  //
   // Rk.: one reason why we need those passes is that we transform the let binding expressions
   // coming from the Dafny ASTs to statements (more specifically, blocks containing variable
   // declarations) in the Dafny-in-Dafny AST. This leads to the introduction of unnecessary
@@ -88,27 +90,193 @@ module Bootstrap.Passes.SimplifyEmptyBlocks {
   import opened Transforms.Generic
   import opened Transforms.Proofs.BottomUp_
 
-  type Expr = Syntax.Expr
+  type {:verify false} Expr = Syntax.Expr
 
-module FilterUtils {
+module FilterCommon {
+  import Utils.Lib
+  import Utils.Lib.Debug
+
   import opened AST.Syntax
-  type Expr = Syntax.Expr
+  import opened Semantics.Equiv
+  import opened Semantics.Interp
+  import opened Transforms.BottomUp // For the def of ``TODO()``
+
+  type {:verify false} Expr = Syntax.Expr
 
   // TODO: move?
-  predicate method IsEmptyBlock(e: Expr)
+  predicate method {:verify false} IsEmptyBlock(e: Expr)
   {
     e.Block? && e.stmts == []
   }
 
   // TODO: move?
-  predicate method IsNonEmptyBlock(e: Expr)
+  predicate method {:verify false} IsNonEmptyBlock(e: Expr)
   {
     !(IsEmptyBlock(e))
   }
 
+  // TODO: move
+  predicate Seq_All<T>(f: T -> bool, s: seq<T>)
+  {
+    forall x | x in s :: f(x)
+  }
+
+  predicate {:verify false} Tr_Expr_Post(e: Expr) {
+    true
+  }
+
+  predicate {:verify false} Tr_Expr_Rel(e: Expr, e': Expr) {
+    EqInterp(e, e')
+  }
+
+
+  // TODO: move
+  predicate {:verify false} EqInterpBlockExprs(es: seq<Exprs.T>, es': seq<Exprs.T>)
+  {
+    Seq_All(SupportsInterp, es) ==>
+    (&& Seq_All(SupportsInterp, es')
+     && forall env, ctx, ctx' | EqState(ctx, ctx') ::
+       EqInterpResultValue(
+                      InterpBlock_Exprs(es, env, ctx),
+                      InterpBlock_Exprs(es', env, ctx')))
+  }
+
+  // TODO: move
+  lemma {:verify false} EqInterpBlockExprs_Inst(es: seq<Exprs.T>, es': seq<Exprs.T>, env: Environment, ctx: State, ctx': State)
+    requires EqInterpBlockExprs(es, es')
+    requires Seq_All(SupportsInterp, es)
+    requires EqState(ctx, ctx')
+    ensures  EqInterpResultValue(InterpBlock_Exprs(es, env, ctx), InterpBlock_Exprs(es', env, ctx'))
+  {}
+  
+  // TODO: move
+  lemma {:verify false} InterpBlock_Exprs_Eq_Append(e: Expr, e': Expr, tl: seq<Expr>, tl': seq<Expr>, env: Environment, ctx: State, ctx': State)
+    requires SupportsInterp(e)
+    requires SupportsInterp(e')
+    requires Seq_All(SupportsInterp, tl)
+    requires Seq_All(SupportsInterp, tl')
+    requires EqState(ctx, ctx')
+    requires EqInterp(e, e')
+    requires EqInterpBlockExprs(tl, tl')
+    requires |tl| > 0
+    ensures EqInterpResultValue(InterpBlock_Exprs([e] + tl, env, ctx), InterpBlock_Exprs([e'] + tl', env, ctx'))
+    // Auxiliary lemma for the proofs about transformations operating on blocks. This is especially
+    // useful when those transformations might update the length of the sequence of expressions
+    // in the blocks. The proof is a bit tricky, because the case where the sequence has length 1
+    // is a special case in the definition of ``EqInterpBlock_Exprs``.
+  {
+    var es := [e] + tl;
+    var es' := [e'] + tl';
+    assert e == es[0];
+
+    reveal InterpBlock_Exprs();
+
+    // Evaluate the first expression
+    var res0 := InterpExpr(e, env, ctx);
+    var res0' := InterpExpr(e', env, ctx');
+    EqInterp_Lem(e, e', env, ctx, ctx');
+
+    // We need to make a case disjunction on whether the length of the concatenated sequences is
+    // > 1 or not
+    if |tl'| >= 1 {
+      // The "regular" case
+
+      // Evaluate the remaining expressions
+      if res0.Success? && res0.value.ret == V.Unit {
+        var Return(_, ctx0) := res0.value;
+        var Return(_, ctx0') := res0'.value;
+
+        var res1 := InterpBlock_Exprs(tl, env, ctx0);
+        var res1' := InterpBlock_Exprs(tl', env, ctx0');
+
+        EqInterpBlockExprs_Inst(tl, tl', env, ctx0, ctx0');
+      }
+      else {
+        // Trivial
+      }
+    }
+    else {
+      // Degenerate case
+      assert |tl'| == 0;
+
+      if res0.Success? {
+        var Return(v, ctx0) := res0.value;
+        var Return(v', ctx0') := res0'.value;
+
+        if v == V.Unit {
+          assert v' == V.Unit;
+          EqInterpBlockExprs_Inst(tl, tl', env, ctx0, ctx0');
+        }
+        else {
+          assert v' != V.Unit;
+
+          // TODO(SMH): update EqInterp so that this works (evaluating `es` will fail if `e` doesn't
+          // evaluate to `Unit`)
+          assume TODO();
+        }
+      }
+      else {
+        // Trivial
+      }
+    }
+  }
+
+  // TODO: move
+  predicate EqInterpResultValue_Strong(res: InterpResult<WV>, res': InterpResult<WV>) {
+    match (res, res') {
+      case (Success(Return(v,ctx)), Success(Return(v',ctx'))) =>
+        && v == v'
+        && ctx == ctx'
+      case (Failure(err), Failure(err')) =>
+        err == err'
+      case _ =>
+        false
+    }
+  }
+
+  // TODO: move
+  // TODO: remove? This lemma is trivial.
+  lemma {:verify false} InterpBlock_Exprs1_Strong_Eq(e: Expr, env: Environment, ctx: State)
+    requires SupportsInterp(e)
+    ensures EqInterpResultValue_Strong(InterpExpr(e, env, ctx), InterpBlock_Exprs([e], env, ctx))
+    // Auxiliary lemma: evaluating a block of one expression is equivalent to evaluating
+    // the single expression.
+  {
+    reveal InterpBlock_Exprs();
+  }
+
+  // TODO: move
+  lemma {:verify false} InterpBlock_Exprs_Refl(es: seq<Expr>, env: Environment, ctx: State, ctx': State)
+    requires Seq_All(SupportsInterp, es)
+    requires EqState(ctx, ctx')
+    ensures EqInterpResultValue(InterpBlock_Exprs(es, env, ctx), InterpBlock_Exprs(es, env, ctx'))
+  {
+    reveal InterpBlock_Exprs();
+    if es == [] {}
+    else {
+       // Evaluate the first expression
+      var res0 := InterpExpr(es[0], env, ctx);
+      var res0' := InterpExpr(es[0], env, ctx');
+      EqInterp_Refl_Lem(es[0]);
+      EqInterp_Lem(es[0], es[0], env, ctx, ctx');
+
+      // Evaluate the remaining expressions
+      if res0.Success? && res0.value.ret == V.Unit {
+        var Return(_, ctx0) := res0.value;
+        var Return(_, ctx0') := res0'.value;
+
+        InterpBlock_Exprs_Refl(es[1..], env, ctx0, ctx0');
+      }
+      else {
+        // Trivial
+      }
+    }
+  }
 }
 
 module FilterEmptyBlocks {
+  // Tranformation 1
+  
   import Utils.Lib
   import Utils.Lib.Debug
   import opened Utils.Lib.Datatypes
@@ -122,16 +290,18 @@ module FilterEmptyBlocks {
   import opened Transforms.Generic
   import opened Transforms.Proofs.BottomUp_
 
-  import opened FilterUtils
+  import opened FilterCommon
 
-  type Expr = Syntax.Expr
+  type {:verify false} Expr = Syntax.Expr
 
-  function method FilterEmptyBlocks_Seq(es : seq<Expr>): seq<Expr>
+  function method {:verify false} FilterEmptyBlocks_Seq(es: seq<Expr>): (es': seq<Expr>)
+    ensures Seq_All(SupportsInterp, es) ==> Seq_All(SupportsInterp, es')
+    ensures |es| >= |es'|
   {
     Seq.Filter(es, IsNonEmptyBlock)
   }
 
-  function method FilterEmptyBlocks_Single(e: Expr): Expr
+  function method {:verify false} FilterEmptyBlocks_Single(e: Expr): Expr
   {
     if e.Block? then
       Expr.Block(FilterEmptyBlocks_Seq(e.stmts))
@@ -139,19 +309,10 @@ module FilterEmptyBlocks {
       e
   }
 
-  predicate Tr_Expr_Post(e: Expr) {
-    true
-  }
-
-  predicate Tr_Expr_Rel(e: Expr, e': Expr) {
-    EqInterp(e, e')
-  }
-
-  lemma FilterEmptyBlocks_Seq_Rel(es: seq<Expr>, env: Environment, ctx: State, ctx': State)
-    requires forall e | e in es :: SupportsInterp(e)
+  lemma {:verify false} FilterEmptyBlocks_Seq_Rel(es: seq<Expr>, env: Environment, ctx: State, ctx': State)
+    requires Seq_All(SupportsInterp, es)
     requires EqState(ctx, ctx')
     ensures EqInterpResultValue(InterpBlock_Exprs(es, env, ctx), InterpBlock_Exprs(FilterEmptyBlocks_Seq(es), env, ctx'))
-    ensures forall e | e in FilterEmptyBlocks_Seq(es) :: SupportsInterp(e)
   {
     reveal InterpBlock_Exprs();
     reveal Seq.Filter();
@@ -161,8 +322,31 @@ module FilterEmptyBlocks {
     var res := InterpBlock_Exprs(es, env, ctx);
     var res' := InterpBlock_Exprs(es', env, ctx');
 
+    // TODO(SMH): there are too many subcases below: I'm pretty sure we can make the proofs in
+    // a smarter way.
     if es == [] {
       // Trivial
+    }
+    else if |es| == 1 {
+      assert es == [es[0]];
+      reveal InterpExpr();
+      reveal InterpBlock();
+      if IsEmptyBlock(es[0]) {
+        assert es' == [];
+
+        // Interp(es, ctx) == ((), ctx)
+        assert InterpBlock_Exprs([es[0]], env, ctx) == InterpExpr(es[0], env, ctx);
+        assert InterpExpr(es[0], env, ctx) == InterpBlock_Exprs(es[0].stmts, env, ctx);
+        assert InterpBlock_Exprs(es[0].stmts, env, ctx) == Success(Return(V.Unit, ctx));
+
+        // Interp(es', ctx') == ((), ctx')
+        assert InterpBlock_Exprs(es', env, ctx') == Success(Return(V.Unit, ctx'));
+      }
+      else {
+        assert es' == es;
+        EqInterp_Refl_Lem(es[0]);
+        EqInterp_Lem(es[0], es[0], env, ctx, ctx');
+      }
     }
     else {
       // Case disjunction: is the first expression in the sequence filtered or not?
@@ -184,34 +368,23 @@ module FilterEmptyBlocks {
       else {
         // The first expression is not filtered
 
-        // Evaluate the first expression
-        var res0 := InterpExpr(es[0], env, ctx);
-        var res0' := InterpExpr(es'[0], env, ctx');
-        assert es[0] == es'[0];
         EqInterp_Refl_Lem(es[0]);
         EqInterp_Lem(es[0], es'[0], env, ctx, ctx');
 
-        // Evaluate the remaining expressions
-        if res0.Success? && res0.value.ret == V.Unit {
-          var Return(_, ctx0) := res0.value;
-          var Return(_, ctx0') := res0'.value;
+        var tl := es[1..];
+        var tl' := FilterEmptyBlocks_Seq(tl);
 
-          var res1 := InterpBlock_Exprs(es[1..], env, ctx0);
-          var res1' := InterpBlock_Exprs(es'[1..], env, ctx0');
-
-          assert res1 == res;
-          assert res1' == res';
-
-          FilterEmptyBlocks_Seq_Rel(es[1..], env, ctx0, ctx0');
+        forall env, ctx, ctx' | EqState(ctx, ctx')
+          ensures EqInterpResultValue(InterpBlock_Exprs(tl, env, ctx), InterpBlock_Exprs(tl', env, ctx'))
+        {
+          FilterEmptyBlocks_Seq_Rel(tl, env, ctx, ctx');
         }
-        else {
-          // Trivial
-        }
+        InterpBlock_Exprs_Eq_Append(es[0], es[0], tl, tl', env, ctx, ctx');
       }
     }
   }
 
-  lemma FilterEmptyBlocks_Single_Rel(e: Expr)
+  lemma {:verify false} FilterEmptyBlocks_Single_Rel(e: Expr)
     ensures Tr_Expr_Rel(e, FilterEmptyBlocks_Single(e))
   {
     if e.Block? && SupportsInterp(e) {
@@ -221,8 +394,139 @@ module FilterEmptyBlocks {
       var es := e.stmts;
 
       forall env, ctx, ctx' | EqState(ctx, ctx')
-        ensures EqInterpResultValue(InterpExpr(e, env, ctx), InterpExpr(e', env, ctx')) {
+        ensures EqInterpResultValue(InterpExpr(e, env, ctx), InterpExpr(e', env, ctx'))
+      {
           FilterEmptyBlocks_Seq_Rel(es, env, ctx, ctx');
+          reveal InterpExpr();
+          reveal InterpBlock();
+      }
+
+      assert SupportsInterp(e');
+      assert EqInterp(e, e');
+    }
+    else {
+      EqInterp_Refl_Lem(e); 
+    }
+  }
+}
+
+module InlineLastBlock {
+  // Tranformation 2
+  
+  import Utils.Lib
+  import Utils.Lib.Debug
+  import opened Utils.Lib.Datatypes
+  import opened Transforms.BottomUp
+
+  import opened AST.Syntax
+  import opened AST.Predicates
+  import opened Semantics.Interp
+  import opened Semantics.Values
+  import opened Semantics.Equiv
+  import opened Transforms.Generic
+  import opened Transforms.Proofs.BottomUp_
+
+  import opened FilterCommon
+
+  type {:verify false} Expr = Syntax.Expr
+
+  function method {:verify false} InlineLastBlock_Seq(es: seq<Expr>): (es': seq<Expr>)
+    ensures Seq_All(SupportsInterp, es) ==> Seq_All(SupportsInterp, es')
+    // If the last expression of a sequence of expressions is a block, inline its content.
+    //
+    // It seems easier to reason about this function if we define it in a recursive way,
+    // which is why we do so.
+  {
+    reveal SupportsInterp();
+
+    // Empty sequence: nothing to do
+    if es == [] then
+      []
+    // We reached the last statement: inline it if it is a block
+    else if |es| == 1 then
+      if es[0].Block? then
+        assert Seq_All(SupportsInterp, es) ==> SupportsInterp(es[0]);
+        assert SupportsInterp(es[0]) ==> Seq_All(SupportsInterp, es[0].stmts);
+        es[0].stmts
+      else
+        [es[0]]
+    // We haven't reached the last element: recurse on the tail
+    else
+      [es[0]] + InlineLastBlock_Seq(es[1..])
+  }
+
+  function method {:verify false} InlineLastBlock_Single(e: Expr): Expr
+  {
+    if e.Block? then Expr.Block(InlineLastBlock_Seq(e.stmts))
+    else e
+  }
+
+  lemma {:verify false} InlineLastBlock_Seq_Rel(es: seq<Expr>, env: Environment, ctx: State, ctx': State)
+    requires forall e | e in es :: SupportsInterp(e)
+    requires EqState(ctx, ctx')
+    ensures forall e | e in InlineLastBlock_Seq(es) :: SupportsInterp(e)
+    ensures EqInterpResultValue(InterpBlock_Exprs(es, env, ctx), InterpBlock_Exprs(InlineLastBlock_Seq(es), env, ctx'))
+  {
+    reveal InterpBlock_Exprs();
+    //reveal Seq.Filter();
+
+    var es' := InlineLastBlock_Seq(es);
+
+    var res := InterpBlock_Exprs(es, env, ctx);
+    var res' := InterpBlock_Exprs(es', env, ctx');
+
+    if es == [] {
+      // Trivial
+    }
+    else if |es| == 1 {
+      if es[0].Block? {
+        reveal InterpExpr();
+        reveal InterpBlock();
+
+        // Doesn't work without this assertion - is it because of the fuel?
+        assert res == InterpExpr(es[0], env, ctx);
+        assert InterpExpr(es[0], env, ctx) == InterpBlock(es[0].stmts, env, ctx);
+
+        assert es' == es[0].stmts;
+        InterpBlock_Exprs_Refl(es[0].stmts, env, ctx, ctx');
+      }
+      else {
+        assert es == es';
+        InterpBlock_Exprs_Refl(es, env, ctx, ctx');
+      }
+    }
+    else {
+      // The first expression appears in both sequences
+      EqInterp_Refl_Lem(es[0]);
+      EqInterp_Lem(es[0], es'[0], env, ctx, ctx');
+
+      // Prove that the sequence concatenations are evaluated in a similar manner
+      var tl := es[1..];
+      var tl' := InlineLastBlock_Seq(tl);
+
+      forall env, ctx, ctx' | EqState(ctx, ctx')
+        ensures EqInterpResultValue(InterpBlock_Exprs(tl, env, ctx), InterpBlock_Exprs(tl', env, ctx'))
+      {
+        InlineLastBlock_Seq_Rel(tl, env, ctx, ctx');
+      }
+      InterpBlock_Exprs_Eq_Append(es[0], es[0], tl, tl', env, ctx, ctx');
+    }
+  }
+
+  // Rk.: modulo the names, this is exactly the same proof as for ``FilterEmptyBlocks_Single_Rel``
+  lemma {:verify true} InlineLastBlock_Single_Rel(e: Expr)
+    ensures Tr_Expr_Rel(e, InlineLastBlock_Single(e))
+  {
+    if e.Block? && SupportsInterp(e) {
+      reveal SupportsInterp();
+
+      var e' := InlineLastBlock_Single(e);
+      var es := e.stmts;
+
+      forall env, ctx, ctx' | EqState(ctx, ctx')
+        ensures EqInterpResultValue(InterpExpr(e, env, ctx), InterpExpr(e', env, ctx'))
+      {
+          InlineLastBlock_Seq_Rel(es, env, ctx, ctx');
           reveal InterpExpr();
           reveal InterpBlock();
       }
